src/Dafny/examples/sextChallengeProblem1Simplified.i.dfy
@@ -2,142 +2,10 @@ include "../llvm.i.dfy"
 include "../control_flow.i.dfy"
 include "generalInstructions.i.dfy"
 
-module challenge_problem_1_simplified {
+module sext_challenge_problem_1_simplified {
     import opened LLVM_def
     import opened control_flow
     import opened general_instructions
-
-// ; Function Attrs: norecurse nounwind readonly ssp uwtable
-// define i32 @rx_message_routine(i8* nocapture readonly %0) local_unnamed_addr #1 {
-//   %2 = getelementptr inbounds i8, i8* %0, i64 2
-//   %3 = load i8, i8* %2, align 1, !tbaa !4
-//   %4 = zext i8 %3 to i32
-//   %5 = add nuw nsw i32 %4, 10
-//   ret i32 %5
-// }
-
-function method{:opaque} lvm_simple_challenge1(dst:lvm_operand_opr,t:bitWidth,op1:lvm_operand_opr,op2:lvm_operand_opr):lvm_code
-{
-    //getelementptr
-    reveal_IntFits();
-    var void := D(Void);
-    var ptrVar:lvm_operand_opr := D(Void);
-    var index := D(Int(2,IntType(8,false)));
-
-    lvm_Block(lvm_CCons(Ins(GETELEMENTPTR(dst,1,op1,index)),
-              lvm_CCons(Ins(RET(void)),lvm_CNil())))
-    // lvm_Block(lvm_CCons(Ins(GETELEMENTPTR(dst,t,op1,op2)),
-    //           lvm_CCons(Ins(RET(void)),lvm_CNil())))
-
-}
-
-lemma lvm_lemma_simple_challenge1(lvm_b0:lvm_codes, lvm_s0:lvm_state, lvm_sN:lvm_state, 
-            dst:lvm_operand_opr,s:MemState,t:bitWidth,op1:lvm_operand_opr,op2:lvm_operand_opr)
-  returns (lvm_bM:lvm_codes, lvm_sM:lvm_state)
-  
-  requires lvm_require(lvm_b0, lvm_simple_challenge1(dst,t,op1,op2), lvm_s0, lvm_sN,dst)
-  requires lvm_is_dst_opr(dst, lvm_s0)
-  requires lvm_is_src_opr(op1, lvm_s0)
-  requires lvm_get_ok(lvm_s0)
-
-  requires ValidOperand(lvm_s0,op1);
-  requires ValidOperand(lvm_s0,op2);
-  requires OperandContents(lvm_s0,op1).Ptr?;
-  requires OperandContents(lvm_s0,op1).bid in lvm_s0.m.mem; //needed for IsValidBid for valid input
-  requires ValidOperand(lvm_s0,dst)
-//   
-  ensures  lvm_ensure(lvm_b0, lvm_bM, lvm_s0, lvm_sM, lvm_sN,dst)
-  ensures  lvm_get_ok(lvm_sM)
-  ensures ValidOperand(lvm_sM,dst)
-
-  ensures OperandContents(lvm_sM,dst).Ptr?;
-  ensures  OperandContents(lvm_sM, dst) == evalGETELEMENTPTR(lvm_s0.m,1,OperandContents(lvm_s0,op1),Int(2,IntType(8,false)));
-  ensures  lvm_state_eq(lvm_sM, lvm_update_ok(lvm_sM, lvm_update_mem( lvm_sM, lvm_s0)))
-{
-  reveal_lvm_simple_challenge1();
-  reveal_lvm_RET();
-  reveal_ValidData();
-  reveal_evalCodeOpaque();
-  reveal_lvm_code_GetElementPtr();
-  reveal_eval_code();
-
-  assert lvm_simple_challenge1(dst,t,op1,op2).Block?;
-  var getelementins := lvm_simple_challenge1(dst,t,op1,op2).block.hd.ins;
-  assert lvm_simple_challenge1(dst,t,op1,op2) == lvm_b0.hd;
-  // Check getelementins validity
-  assert getelementins.GETELEMENTPTR?;
-  assert ValidState(lvm_s0); 
-  assert MemValid(lvm_s0.m);
-  assert ValidOperand(lvm_s0,getelementins.dst);
-  assert ValidOperand(lvm_s0,getelementins.op1);
-  assert ValidOperand(lvm_s0,getelementins.op2);
-  assert OperandContents(lvm_s0,getelementins.op1).Ptr?;
-  assert OperandContents(lvm_s0,getelementins.op2).Int?;
-  assert !OperandContents(lvm_s0,getelementins.op2).itype.signed;
-  assert IsValidBid(lvm_s0.m,OperandContents(lvm_s0,getelementins.op1).bid);
-  // assert IsValidPtr(lvm_s0.m,OperandContents(lvm_s0,getelementins.op1).bid,OperandContents(lvm_s0,getelementins.op1).offset);
-  // assert OperandContents(lvm_s0,getelementins.op1).offset 
-      //  + (OperandContents(lvm_s0,getelementins.op2).val * getelementins.t)
-        //  < |lvm_s0.m.mem[OperandContents(lvm_s0,getelementins.op1).bid]|;
-  //
-  assert ValidInstruction(lvm_s0,getelementins);
-
-  var lvm_old_s:lvm_state := lvm_s0;
-  var two :=D(Void);
-      // var lvm_old_s:lvm_state := lvm_s0;
-  // assert evalCode(Ins(getelementins), lvm_s0, lvm_sN,dst);
-  assert lvm_s0.ok;
-  assert dst == getelementins.dst;
-  var getPtr := D(evalGETELEMENTPTR(lvm_s0.m,t,OperandContents(lvm_s0,getelementins.op1),OperandContents(lvm_s0,getelementins.op2)));
-  // assert getPtr.Ptr?;
-  // assert IsValidPtr(lvm_s0.m,getPtr.bid,getPtr.offset);
-  assert ValidData(lvm_sN,evalGETELEMENTPTR(lvm_s0.m,t,OperandContents(lvm_s0,getelementins.op1),OperandContents(lvm_s0,getelementins.op2)));
-  assert getPtr.D?;
-  assert getPtr.d == evalGETELEMENTPTR(lvm_s0.m,t,OperandContents(lvm_s0,getelementins.op1),OperandContents(lvm_s0,getelementins.op2));
-  // assert  lvm_sN == lvm_s0;
-  // assert evalUpdate(lvm_s0, getPtr, evalGETELEMENTPTR(lvm_s0.m,t,OperandContents(lvm_s0,getelementins.op1),OperandContents(lvm_s0,getelementins.op2)),lvm_sN);
-
-  // assert evalIns(getelementins,lvm_s0, lvm_sN,dst);
-  assert lvm_s0.ok;
-  // assert eval_code(lvm_Block(lvm_b0), lvm_s0, lvm_sN,dst);
-  // assert evalCode(lvm_Block(lvm_b0), lvm_s0, lvm_sN,dst);
-    assert !lvm_b0.CNil?;
-  // assert exists r' :: evalCode(lvm_b0.hd, lvm_s0, r',dst);
-  // assert lvm_b0.hd.Ins?;
-  assert evalBlock(lvm_b0, lvm_s0, lvm_sN,dst);
-
-  ghost var lvm_ltmp1, lvm_cM:lvm_code, lvm_ltmp2 := lvm_lemma_block(lvm_b0, lvm_s0, lvm_sN,dst);
-  lvm_sM := lvm_ltmp1;
-  lvm_bM := lvm_ltmp2;
-  var lvm_b1:lvm_codes := lvm_get_block(lvm_cM);
-  assert lvm_b1.lvm_CCons?;
-  assert lvm_b1.hd.Ins?;
-  assert lvm_b1.hd.ins.GETELEMENTPTR?;
-  // assert lvm_bM.lvm_CCons?;
-  assert lvm_b1.tl.lvm_CCons?;
-  assert lvm_b1.tl.hd.Ins?;
-  assert lvm_b1.tl.hd.ins.RET?;
-  assert lvm_b1.hd == Ins(GETELEMENTPTR(dst,1,op1,D(Int(2,IntType(8,false)))));
-
-  // ghost var lvm_ltmp3, lvm_b2, lvm_s2 := lvm_lemma_block(lvm_b1, lvm_s0, lvm_sM, dst);
-  ghost var lvm_b2, lvm_s2 := lvm_lemma_GetElementPtr(lvm_b1, lvm_s0, lvm_sM, dst, s,1,op1,D(Int(2,IntType(8,false))));
-  assert OperandContents(lvm_s2, dst) 
-        == evalGETELEMENTPTR(lvm_s0.m,1,OperandContents(lvm_s0,op1),Int(2,IntType(8,false)));
-  // assert lvm_sM.ok;
-  assert lvm_b2.hd.Ins?;
-  assert lvm_b2.hd.ins.RET?;
-  assert lvm_b2.hd.ins == RET(D(Void));
-  
-  ghost var lvm_b3, lvm_s3 := lvm_lemma_Ret(lvm_b2, lvm_s2, lvm_sM, dst, D(Void));
-
-  lvm_sM := lvm_lemma_empty(lvm_s3,lvm_sM);
-
-  assert ValidState(lvm_sM);
-  // lvm_sM := lvm_lemma_empty(lvm_s2,lvm_sM);
-
-  assert evalCode_lax(lvm_cM, lvm_s0, lvm_sM,dst);
-  reveal_evalCodeOpaque();
-}
 
 
 // ----*****-----
@@ -163,11 +31,11 @@ requires IsValidBid(s,op1.d.bid) ==> op1.d.offset + ((Int(2,IntType(8,false))).v
     var ptrVar:lvm_operand_opr := D(Void);
     var index := D(Int(2,IntType(8,false)));
 
-    var largetest := D(Int(4294967295,IntType(4,false)));
+    var largetest := D(Int(2147483647,IntType(4,true)));
 
     lvm_Block(lvm_CCons(Ins(GETELEMENTPTR(dst,1,op1,index)),
               lvm_CCons(Ins(LOAD(dst,s,1,dst)),
-              lvm_CCons(Ins(ZEXT(dst,t,dst,4)),
+              lvm_CCons(Ins(SEXT(dst,t,dst,4)),
               lvm_CCons(Ins(ADD(dst,4,dst,largetest)),
               lvm_CCons(Ins(RET(void)),lvm_CNil()))))))
 
@@ -191,7 +59,7 @@ requires IsValidBid(lvm_s0.m,op1.d.bid) ==> op1.d.offset + ((Int(2,IntType(8,fal
   requires OperandContents(lvm_s0,op1).bid in lvm_s0.m.mem; //needed for IsValidBid for valid input
   requires ValidOperand(lvm_s0,dst);
 //   
-  ensures ValidOperand(lvm_sM,dst)
+    ensures ValidOperand(lvm_sM,dst)
   ensures  lvm_get_ok(lvm_sM)
 
   ensures  !OperandContents(lvm_sM, dst).Void? ==> lvm_ensure(lvm_b0, lvm_bM, lvm_s0, lvm_sM, lvm_sN,dst)
@@ -200,9 +68,11 @@ requires IsValidBid(lvm_s0.m,op1.d.bid) ==> op1.d.offset + ((Int(2,IntType(8,fal
   // ensures  OperandContents(lvm_sM, dst) == evalGETELEMENTPTR(lvm_s0.m,1,OperandContents(lvm_s0,op1),Int(2,IntType(8,false)));
   ensures  !OperandContents(lvm_sM, dst).Void? ==> OperandContents(lvm_sM, dst).Int?;
   ensures  !OperandContents(lvm_sM, dst).Void? ==> OperandContents(lvm_sM, dst).itype.size == 4;
-  ensures  !OperandContents(lvm_sM, dst).Void? ==> OperandContents(lvm_sM, dst).val < 0x1_0000_0000;
-  ensures  !OperandContents(lvm_sM, dst).Void? ==> OperandContents(lvm_sM, dst).val >= 0;
+//   ensures  !OperandContents(lvm_sM, dst).Void? ==> OperandContents(lvm_sM, dst).val < 0x1_0000_0000;
+  ensures  !OperandContents(lvm_sM, dst).Void? ==> OperandContents(lvm_sM, dst).itype.signed;
 
+
+  // evalLOAD(lvm_sM.m,lvm_sN.m,1,evalGETELEMENTPTR(lvm_s0.m,1,OperandContents(lvm_s0,op1),Int(2,IntType(8,false))));
 
   ensures  !OperandContents(lvm_sM, dst).Void? ==> lvm_state_eq(lvm_sM, lvm_update_ok(lvm_sM, lvm_update_mem( lvm_sM, lvm_s0)))
 {
@@ -210,7 +80,7 @@ requires IsValidBid(lvm_s0.m,op1.d.bid) ==> op1.d.offset + ((Int(2,IntType(8,fal
   reveal_lvm_RET();
   reveal_lvm_LOAD();
   reveal_lvm_code_Add();
-  reveal_lvm_code_ZEXT();
+  reveal_lvm_code_SEXT();
   reveal_ValidData();
   reveal_evalCodeOpaque();
   reveal_IntFromBytes();
@@ -302,8 +172,8 @@ requires IsValidBid(lvm_s0.m,op1.d.bid) ==> op1.d.offset + ((Int(2,IntType(8,fal
   //   var x := IntFromBytes(OperandContents(lvm_s3,dst).bytes, IntType(byteSize,false));
   // }else{
     assert lvm_b3.hd.Ins?;
-    assert lvm_b3.hd.ins.ZEXT?;
-    assert lvm_b3.hd.ins == ZEXT(dst,t,dst,4);
+    assert lvm_b3.hd.ins.SEXT?;
+    assert lvm_b3.hd.ins == SEXT(dst,t,dst,4);
     assert lvm_b3.tl.lvm_CCons?;
     assert lvm_b3.tl.hd.Ins?;
     assert lvm_b3.tl.hd.ins.ADD?;
@@ -314,7 +184,7 @@ requires IsValidBid(lvm_s0.m,op1.d.bid) ==> op1.d.offset + ((Int(2,IntType(8,fal
   // requires OperandContents(lvm_s0,dst).Int?;
   // assert !OperandContents(lvm_s3,dst).itype.signed;
 
-    ghost var lvm_b4, lvm_s4 := lvm_lemma_Zext(lvm_b3, lvm_s3, lvm_sM, dst, t,dst,4);
+    ghost var lvm_b4, lvm_s4 := lvm_lemma_Sext(lvm_b3, lvm_s3, lvm_sM, dst, t,dst,4);
     assert OperandContents(lvm_s4, dst).Int?;
 
     assert lvm_s4.ok;
@@ -324,10 +194,15 @@ requires IsValidBid(lvm_s0.m,op1.d.bid) ==> op1.d.offset + ((Int(2,IntType(8,fal
     // assert lvm_b4.hd
 
 //    ghost var lvm_b2, lvm_s2 := lvm_lemma_Add(lvm_b1, lvm_s0, lvm_sM, src2, size,src1,val,o);
-    var largetest := D(Int(4294967295,IntType(4,false)));
+    var largetest := D(Int(2147483647,IntType(4,true)));
 
     ghost var lvm_b5, lvm_s5 := lvm_lemma_Add(lvm_b4, lvm_s4, lvm_sM, dst,4,dst, largetest,dst);
-
+        assert OperandContents(lvm_s5, dst).Int?;
+        assert OperandContents(lvm_s5, dst).itype.signed;
+        assert OperandContents(lvm_s5, dst).val == evalADD(OperandContents(lvm_s4,dst).itype.size,OperandContents(lvm_s4,dst),OperandContents(lvm_s4,largetest)).val;
+        // assert OperandContents(lvm_s5, dst).val >= 2147483647;
+        assert ToTwosComp(OperandContents(lvm_s5, dst)).val == 
+          (OperandContents(lvm_s4, dst).val + OperandContents(lvm_s4, largetest).val) % Pow256(OperandContents(lvm_s4, dst).itype.size);
 
     ghost var lvm_b6, lvm_s6 := lvm_lemma_Ret(lvm_b5, lvm_s5, lvm_sM, dst, D(Void));
 
@@ -339,8 +214,7 @@ requires IsValidBid(lvm_s0.m,op1.d.bid) ==> op1.d.offset + ((Int(2,IntType(8,fal
 
     assert evalCode_lax(lvm_cM, lvm_s0, lvm_sM,dst);
     reveal_evalCodeOpaque();
+  // }
   }
 }
-
-
 }
